[sledge sem] Adds a theorem about block processing order
Summary:
Show that the SSA restrictions imply that the blocks can be
topologically sorted so that any use of a variable follows its
definition in the list of blocks. This showed a slight flaw in my
definition of SSA form. It used to treat program counters up to
equality. However, PCs that point to a block header contain the location
that control came from (so that the Phi instructions can be executed),
but the SSA restrictions shouldn't pay attention to that, so now the
definition of SSA introduces a equivalence on PCs that ignores that
additional information.

Reviewed By: jberdine

Differential Revision: D21066873

fbshipit-source-id: 735575a1f

sledge/semantics/llvmScript.sml
@@ -830,15 +830,15 @@ Definition prog_ok_def:
        alookup p fname = Some dec ⇒
        every (\b. fst b = None ⇔ (snd b).h = Entry) dec.blocks) ∧
      ((* The blocks in a definition have distinct labels.*)
-      ∀fname dec.
-       alookup p fname = Some dec ⇒
-       all_distinct (map fst dec.blocks)) ∧
+      every (\(fname,dec). all_distinct (map fst dec.blocks)) p) ∧
      (* There is a main function *)
      (∃dec. alookup p (Fn "main") = Some dec) ∧
      (* No phi instruction assigns the same register twice *)
      (∀ip from_l phis.
        get_instr p ip (Inr (from_l, phis)) ⇒
-       all_distinct (map (λp. case p of Phi r _ _ => r) phis))
+       all_distinct (map (λp. case p of Phi r _ _ => r) phis)) ∧
+     (* No duplicate function names *)
+     (all_distinct (map fst p))
 End
 
 (* All call frames have a good return address, and the stack allocations of the
